dw/DeepWeb/Lib/SimpleSpec.v
@@ -1,3 +1,6 @@
+Require Import List.
+Import ListNotations.
+
 From QuickChick Require Import QuickChick.
 From Custom Require Import String Monad.
 Import MonadNotations.
@@ -21,8 +24,7 @@ From DeepWeb Require Export
 
 (** ** Server *)
 
-(* Types and operations for defining server implementation ITrees.
-   For more details, see [Lib.SimpleSpec_Server]. *)
+(* Types and operations for defining server implementation ITrees. *)
 Module Type ServerIface.
 
 (* A server is a program with internal nondeterminism and
@@ -66,11 +68,11 @@ Parameter recv_full : connection_id -> nat -> ServerM bytes.
 Parameter send : connection_id -> bytes -> ServerM unit.
 
 End ServerIface.
+(* Implemented in [Lib.SimpleSpec_Server]. *)
 
 (** ** Observer *)
 
-(* Module to define specifications as "observer" ITrees.
-   For more details, see [Lib.SimpleSpec_Observer]. *)
+(* Module to define specifications as "observer" ITrees. *)
 Module Type ObserverIface.
 
 (** The type of observations that can be made. *)
@@ -110,33 +112,117 @@ Definition obs_from_server :
 
 (* Also some derived operations. *)
 
-(* Make an assertion on a value, if it exists. *)
-(* BCP: Think about how to explain this *)
+(* Make an assertion on a value, if it exists.  (If the value is 
+   [Some x] and the test returns false on [x], the [assert_on] 
+   ITree fails. *)
 Parameter assert_on :
   forall {A}, string -> option A -> (A -> bool) -> ObserverM unit.
 
-(* Observe a message of fixed-length sent to the server. *)
+(* Observe a message of fixed length sent to the server. *)
 Parameter obs_msg_to_server : nat -> connection_id -> ObserverM bytes.
 
-(* Observe a message of fixed length received from the server
-   and match it with an expected value, failing if they are not
-   equal. *)
+(* Observe a message of fixed length received from the server and
+   match it with an expected value, failing if they are not
+   equal.  (This is implemented in terms of [obs_from_server] and
+   [assert_on].  In particular, when [obs_from_server] returns [None],
+   we want to assume that the hole stands for the next expected byte
+   and continue past it.) *)
 Parameter obs_msg_from_server : connection_id -> bytes -> ObserverM unit.
 
-(* [obs_msg_from_server] is implemented in terms of [obs_from_server]
-   and [assert_on].  In particular, when [obs_from_server] returns
-   [None], we assume that the hole stands for the next expected
-   byte. *)
-
 End ObserverIface.
+(* Implemented in [Lib.SimpleSpec_Observer]. *)
+
+(** ** Network Model *)
+
+(* BCP: From here on, the "narrative flow" gets a little wobbly... *)
+
+(* The above interfaces describe servers and observers that interact
+   over a network, which we model as the following state machine... *)
+Module Type NetworkModelIface.
+
+(* The network state is a map from [connection_id] to connection
+   states. *)
+
+Section ConnectionState.
+
+(* First, we define the type of a single connection
+   state ([connection_state]).  Essentially, a connection can be seen
+   as a pair of buffers that servers and clients push bytes to
+   asynchronously.
+      - Connections start in the [CLOSED] state.
+      - When a client initiates a connection, the connection enters
+        the [PENDING] state, and the client can immediately start
+        sending messages over it.
+      - The server must then accept the connection, which enters the
+        [ACCEPTED] state, before receiving and sending messages over
+        it. The client can now also receive messages. *)
+
+Inductive connection_state_enum := CLOSED | PENDING | ACCEPTED.
+
+Record connection_state :=
+  Build_connection_state {
+
+    (* The state of the connection (see above). *)
+    connection_status : connection_state_enum;
+
+    (* The buffer of bytes going into the server. *)
+    connection_inbytes : list byte;
+
+    (* The buffer of bytes going out from the server. *)
+    connection_outbytes : list byte;
+  }.
+
+Definition initial_cs : connection_state := {|
+    connection_status := CLOSED;
+    connection_inbytes := [];
+    connection_outbytes := [];
+  |}.
+
+End ConnectionState.
+
+(* We can now define the complete state of the network
+   as a map from [connection_id] to [connection_state]. *)
+Definition network_state := Map.t connection_id connection_state.
+
+(* Initial state: all connections are closed. *)
+Definition initial_ns : network_state := fun _ => initial_cs.
+
+(* State transitions.
+   - The result is [None] when a transition is not defined.
+   - Transitions may carry some output (in this case, a byte
+     for [recv] transitions. *)
+Definition transition (output : Type) : Type :=
+  network_state -> option (network_state * output).
+
+(* Each of the following possible transitions succeeds (returning a
+   result and a next state) if the given transition is possible from
+   the current network state. *)
+
+(* Server-side transitions *)
+Parameter server_accept : connection_id -> transition unit.
+Parameter server_send : connection_id -> byte -> transition unit.
+Parameter server_recv : connection_id -> transition byte.
+
+(* Client-side transitions *)
+Parameter client_connect : connection_id -> transition unit.
+Parameter client_send : connection_id -> byte -> transition unit.
+Parameter client_recv : connection_id -> transition byte.
+
+End NetworkModelIface.
+(* Implemented in [Lib.SimpleSpec_NetworkModel]. *)
 
 (** ** Event traces *)
 
-Module Type TracesIface.
+Module Type TracesIface (NetworkModel : NetworkModelIface).
 
-(* An event can be observed to happen on the network, either from the
-   server's or the client's point of view.  It is paremeterized by the
-   type to represent the server's output... *)
+(* The refinement relation between ITrees is stated in terms of _event
+   traces_, which are simply lists of events.
+
+   Events are parameterized by the type to represent the server's
+   output. For specification purposes, an output is a plain
+   [byte] ([real_event]). But for testing it will be useful to insert
+   holes by instantiating [byte' := option byte]. *)
+
 Inductive event (byte' : Type) :=
 | NewConnection : connection_id -> event byte'
 | ToServer : connection_id -> byte -> event byte'
@@ -145,69 +231,138 @@ Inductive event (byte' : Type) :=
 (* Traces are sequences of events. *)
 Definition trace byte' := list (event byte').
 
-(* ... In the real world, this output is a concrete byte. *)
+(* In the real world, events carry concrete bytes. *)
 Definition real_event := event byte.
 Definition real_trace := list real_event.
 
-(* ... but it is also useful for testing to insert hypothetical bytes
-   of unknown values in a trace, representing values that the server
-   may have output but which have not reached the client yet. *)
+(* For testing, it is useful to insert "hypothetical bytes" of unknown
+   values in a trace, representing values that the server may have
+   output but which have not reached the client yet. *)
 Definition hypo_event := event (option byte).
 Definition hypo_trace := list hypo_event.
 
-Parameter real_to_hypo : real_trace -> hypo_trace.
+(* Traces with holes are a superset of real traces. *)
+(* BCP: Do we need these in the interface? *)
+Parameter real_to_hypo_trace : real_trace -> hypo_trace.
+Coercion real_to_hypo_trace : real_trace >-> hypo_trace.
 
-(* [is_server_trace server tr] holds if [tr] is a trace of
-   the [server].  *)
+(* [is_server_trace server tr] holds if [tr] is a trace of the [server].  *)
 Parameter is_server_trace : ServerM unit -> real_trace -> Prop.
 
 (* [is_observer_trace observer tr] holds if [tr] is a trace of
-   the [observer]. *)
+   the [observer]; [tr] may contain holes. *)
 Parameter is_observer_trace : ObserverM unit -> hypo_trace -> Prop.
 
-(* Corresponding "server-side" and "client-side" traces. *)
-Parameter network_scrambled : real_trace -> real_trace -> Prop.
+(* These events label transitions in the network state machine
+   defined above in [NetworkModelIface]. *)
 
-(* Property that a real trace [tr] is a scrambled trace of some
-   spec trace. *)
+Import NetworkModel.
+
+(* Server-side interpretation of an event. *)
+Definition server_transition (ev : real_event)
+                           : network_state -> network_state -> Prop :=
+  fun ns ns' =>
+    match ev with
+    | NewConnection c => server_accept c ns = Some (ns', tt)
+    | ToServer c b => server_recv c ns = Some (ns', b)
+    | FromServer c b => server_send c b ns = Some (ns', tt)
+    end.
+
+(* Client-side interpretation of an event. *)
+Definition client_transition (ev : real_event) :
+  network_state -> network_state -> Prop :=
+  fun ns ns' =>
+    match ev with
+    | NewConnection c => client_connect c ns = Some (ns', tt)
+    | ToServer c b => client_send c b ns = Some (ns', tt)
+    | FromServer c b => client_recv c ns = Some (ns', b)
+    end.
+
+(* The main "scrambling" relation. *)
+(* [network_scrambled_ ns tr str] holds when, starting from
+   the network state [ns], there is an execution of the
+   network with server-side trace [tr_server] and client-side
+   trace [tr_client].
+
+   We say that [tr_client] is a scrambling of [tr_server],
+   or that [tr_server] is a descrambling of [tr_client]. *)
+Inductive network_scrambled_
+                : network_state -> real_trace -> real_trace -> Prop :=
+| ScrambleEmpty : forall ns, network_scrambled_ ns [] []
+| ScrambleServer : forall ns ns' e tr_server tr_client,
+    server_transition e ns ns' ->
+    network_scrambled_ ns'       tr_server  tr_client ->
+    network_scrambled_ ns  (e :: tr_server) tr_client
+| ScrambleClient : forall ns ns' e tr_server tr_client,
+    client_transition e ns ns' ->
+    network_scrambled_ ns' tr_server       tr_client ->
+    network_scrambled_ ns  tr_server (e :: tr_client).
+
+(* At the top level, we consider traces starting from the initial state. *)
+Definition network_scrambled := network_scrambled_ initial_ns.
+
+(* A trace [str] is "consistent" with an [observer] if it can be
+   descrambled to an [observer] trace. We say that [str] is a
+   "scrambled trace" of [observer]. *)
 Definition is_scrambled_trace : ObserverM unit -> real_trace -> Prop :=
   fun observer tr =>
     exists str,
       network_scrambled str tr /\
-      is_observer_trace observer (real_to_hypo str).
+      is_observer_trace observer str.
 
-(* A server ([server : ServerM unit]) refines a "linear spec"
-   ([observer : ObserverM unit]) if, for every trace [tr] that the
-   server can produce, and every trace [str] that can be observed
-   from it via the network, it can be explained by a "descrambled
-   trace" [dstr] in the "linear spec".
-   Some examples can be found in [Spec/Swap_ExampleServers.v].
- *)
-Parameter refines_mod_network :
-  ObserverM unit -> ServerM unit -> Prop.
+(* The main property defining our notion of "correctness". *)
+
+(* Refinement relation "modulo network scrambling".
+
+   A server ([server : ServerM unit]) refines a "linear spec"
+   (an [observer : ObserverM unit]) if, for every trace [tr] that the
+   server can produce, and every scrambling [str] of [tr]
+   (representing what we observe of [tr] from the other side of
+   the network), [str] is a scrambled trace of the [observer].
+   Some examples can be found in [Spec.Descramble_Examples]. *)
+Definition refines_mod_network observer server : Prop :=
+  forall tr : real_trace,
+    is_server_trace server tr ->
+    forall str : real_trace,
+      network_scrambled tr str ->
+      exists dstr : real_trace,
+        network_scrambled dstr str /\
+        is_observer_trace observer dstr.
 
 (* Tests *)
 
-(* See [Lib.Util.result] for the definition of the test result
-   types below. *)
+(* [Lib.Util.result] (from which [Lib.Util.simple_result] and
+   [descrambled_result] are derived) is a type with three
+   constructors representing success, failure, or "don't know",
+   possibly with a (counter)example. *)
 
 (* A test for [is_observer_trace]. *)
-(* TODO: reuse comment above the definition of this thing? *)
 Parameter is_observer_trace_test :
-  nat -> ObserverM unit -> hypo_trace -> simple_result.
+  ObserverM unit -> hypo_trace -> simple_result.
 
-(* Test result of descrambling: if a descrambling is found,
-   it gets returned. *)
+(* Test result of descrambling: success is witnessed by a
+   descrambled [hypo_trace]. *)
 Definition descrambled_result := result hypo_trace unit.
 
-(* A test for [is_scrambled_trace]. *)
+(* A test for [is_scrambled_trace], which tries to
+   descramble the given trace to a trace of the observer. *)
 Parameter is_scrambled_trace_test :
-  nat -> ObserverM unit -> real_trace -> descrambled_result.
+  ObserverM unit -> real_trace -> descrambled_result.
 
 (* A test for [refines_mod_network].
    Check that every trace of the server can be descrambled into
-   a trace of the spec. *)
+   a trace of the observer. *)
 Parameter refines_mod_network_test :
   ObserverM unit -> ServerM unit -> Checker.
 
 End TracesIface.
+(* The implementation of this interface is split in a couple of modules.
+   The most important parts:
+   - the definition of events and descrambling is in
+     [Lib.SimpleSpec_Traces];
+   - the general property [refines_mod_network] is defined in
+     [Lib.SimpleSpec_Refinement];
+   - the descrambling function for a single trace,
+     [is_scrambled_trace_test] is in [Lib.SimpleSpec_Descramble];
+   - the test function for refinement, [refines_mod_network_test]
+     is in [Lib.SimpleSpec_ServerTrace]. *)
