dw/DeepWeb/Spec/Descramble_Examples.v
@@ -1,0 +1,377 @@
+(*! Section SwapExamples *)
+
+Generalizable Variable E.
+Typeclasses eauto := 6.
+
+From QuickChick Require Import QuickChick.
+
+Require Import Ascii String List PArith.
+Require Fin.
+Import ListNotations.
+
+From Custom Require Import String.
+
+Require Import DeepWeb.Free.Monad.Free.
+Import MonadNotations.
+Require Import DeepWeb.Free.Monad.Common.
+Import SumNotations.
+
+Require Import DeepWeb.Lib.Util DeepWeb.Lib.SimpleSpec.
+
+Require Import DeepWeb.Spec.Swap_SimpleSpec.
+
+(* begin hide *)
+Set Warnings "-extraction-opaque-accessed,-extraction".
+Open Scope string_scope.
+(* end hide *)
+
+(* BCP: Too much boilerplate!
+
+    refines_mod_network_test
+      swap_observer_def (bounded_server Def.buffer_size [] Def.init_message).
+*)
+
+Import EventNotations.
+
+(** * Example scrambled traces *)
+
+(* BCP: linear -> server *) (* LY: is this better? *)
+(* "Scrambled traces" describe what the clients _across the network_
+   can observe, given that the server is behaving according to the
+   given sequential specification.
+
+   The [is_scrambled_trace_test] function checks whether a given
+   "observed trace" is a scrambled version of a trace belonging
+   to a given specification.  If so, it returns that "descrambled
+   trace" that explains the observed trace. *)
+
+(* Every actual trace of the server is also a scrambled trace: *)
+Example scrambled_trace_example_1 :
+  is_scrambled_trace_test swap_observer_def [
+    0 !;
+    1 !;
+    0 <-- "a";
+    0 <-- "b";
+    0 <-- "c";
+    0 --> "0";
+    0 --> "0";
+    0 --> "0";
+    1 <-- "d";
+    1 <-- "e";
+    1 <-- "f";
+    1 --> "a";
+    1 --> "b";
+    1 --> "c"
+  ]%real = OK [
+    0 !;
+    1 !;
+    0 <-- "a";
+    0 <-- "b";
+    0 <-- "c"; 
+    0 --> "0";
+    0 --> "0";
+    0 --> "0";
+    1 <-- "d"; 
+    1 <-- "e";
+    1 <-- "f";
+    1 --> "a";
+    1 --> "b"; 
+    1 --> "c"
+  ]%hypo.
+Proof. cbn. reflexivity. Qed.
+
+(* The "scrambling" of messages in the network can result in responses
+   on different connections being received out of order.  The
+   resulting "explanation" shows the order that they must have been
+   sent by the server. *)
+Example scrambled_trace_example_2 :
+  is_scrambled_trace_test swap_observer_def [
+    0 !;
+    1 !;
+    0 <-- "a";
+    0 <-- "b";
+    0 <-- "c";
+    1 <-- "d";
+    1 <-- "e";
+    1 <-- "f";
+    1 --> "a";
+    1 --> "b";
+    1 --> "c";
+    0 --> "0";
+    0 --> "0";
+    0 --> "0"
+  ]%real = OK [
+    0 !;
+    1 !;
+    0 <-- "a";
+    0 <-- "b";
+    0 <-- "c";
+    0 --> "0";
+    0 --> "0";
+    0 --> "0";
+    1 <-- "d";
+    1 <-- "e";
+    1 <-- "f";
+    1 --> "a";
+    1 --> "b";
+    1 --> "c"]%hypo.
+Proof. reflexivity. Qed.
+
+(* A bad trace, where the server sends back a response that was never
+   sent to it by any client: *)
+Example bad_scrambled_trace_example_1 :
+  is_scrambled_trace_test swap_observer_def [
+    0 !;
+    0 <-- "a";
+    0 <-- "b";
+    0 <-- "c";
+    0 --> "X"
+  ]%real = FAIL tt.
+Proof. reflexivity. Qed.
+
+(* A more interesting bad trace, where the server appears to send the
+   requests from connection 1 as responses along connection 2 _and
+   vice versa_. *)
+Example bad_scrambled_trace_example_2 :
+  is_scrambled_trace_test swap_observer_def [
+    0 !;
+    1 !;
+    2 !;
+    0 <-- "a";
+    0 <-- "b";
+    0 <-- "c";
+    1 <-- "d";
+    1 <-- "e";
+    1 <-- "f";
+    2 <-- "g";
+    2 <-- "h";
+    2 <-- "i";
+    1 --> "g";
+    1 --> "h";
+    1 --> "i";
+    2 --> "d";
+    2 --> "e";
+    2 --> "f"
+  ]%real = FAIL tt.
+Proof. reflexivity. Qed.
+
+(* Finally, an example of a trace that might be observed if the
+   responses on connection 1 are delayed by the network.  The
+   explanation of this observation includes three "hypothetical
+   events" on connection 1, marking places where a client is still
+   expecting messages from the server. *)
+Example scrambled_trace_example_3 :
+  is_scrambled_trace_test swap_observer_def [
+    0 !;
+    1 !;
+    0 <-- "a";
+    0 <-- "b";
+    0 <-- "c";
+    1 <-- "d";
+    1 <-- "e";
+    1 <-- "f";
+    0 --> "d";
+    0 --> "e";
+    0 --> "f"
+  ]%real = OK [
+    0 !;
+    1 !;
+    1 <-- "d";
+    1 <-- "e";
+    1 <-- "f";
+    1 --> ?;
+    1 --> ?;
+    1 --> ?;
+    0 <-- "a";
+    0 <-- "b";
+    0 <-- "c";
+    0 --> "d";
+    0 --> "e";
+    0 --> "f"]%hypo.
+Proof. reflexivity. Qed.
+
+(* The reason for including these "hypothetical events" in
+   explanations is that it enables us to reject observations like
+   this, where three "missing" events are followed by one that is
+   clearly impossible: *)
+Example bad_scrambled_trace_example_3 :
+  is_scrambled_trace_test swap_observer_def [
+    0 !;
+    1 !;
+    0 <-- "a";
+    0 <-- "b";
+    0 <-- "c";
+    1 <-- "d";
+    1 <-- "e";
+    1 <-- "f";
+    0 --> "0";
+    1 --> "X"
+  ]%real = FAIL tt.
+Proof. reflexivity. Qed.
+
+(** * Refinement-modulo-descrambling examples *)
+
+(** ** Straightforward swap server *)
+
+(* A swap server that trivially follows the specification. *)
+
+CoFixpoint swap_server_loop (buffer_size : nat)
+                          (conns : list connection_id)
+                          (last_msg : bytes) 
+                        : ServerM unit :=
+  disj
+    ( (* Accept a new connection. *)
+      c <- accept;;
+      swap_server_loop buffer_size (c :: conns) last_msg
+    | (* Exchange a pair of messages on a connection. *)
+      c <- choose conns;;
+      msg <- recv c buffer_size;;
+      send c last_msg;;
+      swap_server_loop buffer_size conns msg
+    )%nondet.
+
+Definition swap_server_def : ServerM unit :=
+  swap_server_loop Def.buffer_size [] Def.init_message.
+
+Definition test_swap := refines_mod_network_test
+                          swap_observer_def swap_server_def.
+
+(*! QuickChick test_swap. *)
+
+(* QuickChecking test_swap +++ Passed 10000 tests (0 discards) *)
+
+(** ** Trivial server *)
+
+(* A silly server that does no useful work at all (it accepts
+   connections but never sends or receives on them) *)
+CoFixpoint eager_server (tt : unit) : ServerM unit :=
+  c <- accept ;;
+  eager_server tt.
+
+Definition test_eager := refines_mod_network_test
+                           swap_observer_def (eager_server tt).
+
+(*! QuickChick test_eager. *)
+
+(* QuickChecking test_eager ++ Passed 10000 tests (0 discards) *)
+
+(** ** Bad server *)
+
+(* A server that's plainly wrong. *)
+
+CoFixpoint const_server (buffer_size : nat) : ServerM unit :=
+  c <- accept ;;
+  msg <- recv c buffer_size ;;
+  send c "0";;
+  const_server buffer_size.
+
+Definition test_const :=
+  expectFailure
+    (refines_mod_network_test
+       swap_observer_def (const_server Def.buffer_size)).
+
+(*! QuickChick test_const. *)
+(* ===>
+     QuickChecking test_const
+[[
+     [1 !; 1 <-- "C"; 1 <-- "\022"; 1 <-- "\003"; 1 --> "0"; 
+      2 !; 2 <-- "P"; 2 <-- "o"; 2 <-- "n"; 2 --> "0"]
+]]
+     *** Failed after 1 tests and 0 shrinks. (0 discards) *)
+
+(** ** Bounded server *)
+
+(* A (correct) server that only accepts up to two connections *)
+
+CoFixpoint bounded_server (buffer_size : nat) 
+                          (conns : list connection_id)
+                          (last_msg : string)
+                        : ServerM unit :=
+  disj
+     ( if (length conns <= 2)? then
+         c <- accept ;; bounded_server buffer_size (c :: conns) last_msg
+       else
+         ret tt ;; bounded_server buffer_size conns last_msg
+     | c <- choose conns;;
+       msg <- recv c buffer_size ;;
+       send c last_msg ;;
+       bounded_server buffer_size conns msg 
+     )%nondet.
+
+Definition test_bounded_server :=
+  refines_mod_network_test
+    swap_observer_def (bounded_server Def.buffer_size [] Def.init_message).
+
+(*! QuickChick test_bounded_server. *)
+
+(** ** Terminating server *)
+
+(* A server that works for a while and then stops. *)
+
+CoFixpoint terminating_server (buffer_size : nat) (conns : list connection_id)
+                              (last_msg : string) (num_sends : nat) 
+                            : ServerM unit :=
+  if num_sends < 3 ? then 
+    disj
+      ( c <- accept;;
+        terminating_server buffer_size (c :: conns) last_msg num_sends
+      | c <- choose conns;;
+        msg <- recv c buffer_size;;
+        send c last_msg;;
+        terminating_server buffer_size conns msg (num_sends + 1)
+      )%nondet
+  else ret tt.
+
+Definition test_terminating_server :=
+  refines_mod_network_test
+    swap_observer_def
+    (terminating_server Def.buffer_size [] Def.init_message 0).
+
+(*! QuickChick test_terminating_server. *)
+
+(* BCP: Put in all QC results in comments, with ===>.  Comment on lack
+   of shrinking. *)
+
+(** ** Eventually bad server *)
+
+(* A server that behaves properly at first, then malfunctions. *)
+Definition malfunctioning_server 
+                 (buffer_size : nat) (conns : list connection_id)
+                 (last_msg : string) (num_sends : nat) 
+               : ServerM unit :=
+  terminating_server buffer_size conns last_msg num_sends ;;
+  const_server buffer_size.
+  
+Definition test_malfunctioning_server :=
+  expectFailure
+    (refines_mod_network_test
+      swap_observer_def
+      (malfunctioning_server Def.buffer_size [] Def.init_message 0)).
+
+(*! QuickChick test_malfunctioning_server. *)
+
+(** ** Echo server *)
+
+(* BCP: Why the unit arguments?  For extraction?? *)
+
+(* Finally, just to show that we can specify things besides swap
+   servers (;-), here is a simple echo server that repeatedly accepts
+   a connection, receives up to 2 bytes, and sends them back along the
+   same connection. *)
+
+CoFixpoint echo (tt : unit) : ServerM unit :=
+  c <- accept ;;
+  msg <- recv c 2 ;;
+  send c msg ;;
+  echo tt.
+
+CoFixpoint echo_spec (tt : unit) : ObserverM unit :=
+  c <- obs_connect ;;
+  msg <- obs_msg_to_server 2 c;;
+  obs_msg_from_server c msg ;;
+  echo_spec tt.
+
+Definition test_echo := refines_mod_network_test (echo_spec tt) (echo tt).
+
+(*! QuickChick test_echo. *)
+
