dw/DeepWeb/Spec/Swap_CLikeSpec.v
@@ -112,17 +112,27 @@ Definition has_conn_state {A} `{HasConnectionState A}
 Definition is_complete (buffer_size : Z) (msg : string) :=
   Z.eqb (Z.of_nat (String.length msg)) buffer_size.
 
+(* Wait for a message from connection [conn].
+   [recv] can return a partial message, in which case we store the
+   bytes we received to try receiving more in a late. iteration. *)
 Definition conn_read (buffer_size : Z)
            (conn: connection) (last_full_msg : string)
   : M socketE (connection * string) :=
   let req_len := Z.of_nat (String.length (conn_request conn)) in
   or (r <- recv (conn_id conn) (Z.to_nat (buffer_size - req_len)) ;;
       match r with
+        (* If [recv] returns [r = None], the connection was closed. *)
       | None => ret (upd_conn_state conn DELETED, last_full_msg)
+        (* Otherwise, we append the received bytes to the other
+           bytes previously received on that connection. *)
       | Some msg =>
         let msg_len := Z.of_nat (String.length msg) in
         let msg' := (*!*) (conn_request conn ++ msg)%string (*! "BAD" *) in
         if is_complete buffer_size msg' then
+          (* If the client's message is complete (i.e., of
+             length [buffer_size]) we prepare to respond with
+             [last_full_msg] and store the [msg'] for the next
+             exchange. *)
           let conn' :=  {| conn_id := conn_id conn ;
                            conn_request := msg';
                            conn_response := last_full_msg;
@@ -131,6 +141,7 @@ Definition conn_read (buffer_size : Z)
                         |}
           in ret (conn', msg')
         else
+          (* Otherwise we wait for more input from this connection. *)
           let conn' := {| conn_id := conn_id conn ;
                           conn_request := msg';
                           conn_response := conn_response conn;
@@ -142,6 +153,11 @@ Definition conn_read (buffer_size : Z)
      )
      (ret (conn, last_full_msg)).
 
+(* Send a response on connection [conn].
+   [send_any_prefix] (representing the [send] POSIX syscall)
+   may send only a prefix of the message (it returns the length [r]
+   of that prefix), in which case we will retry sending the rest
+   in a later iteration. *)
 Definition conn_write (conn: connection) : M socketE connection :=
   or (let num_bytes_sent := Z.to_nat (conn_response_bytes_sent conn) in
       r <- send_any_prefix
@@ -149,17 +165,24 @@ Definition conn_write (conn: connection) : M socketE connection :=
             (substring num_bytes_sent
                        (String.length (conn_response conn) - num_bytes_sent)
                        (conn_response conn)) ;;
-      if (String.length (conn_response conn) <? r)%nat then fail "dead code"
+      if (String.length (conn_response conn) <? r)%nat
+      then
+        (* The sent prefix [r] must be no longer than the actual
+           message to send. *)
+        fail "dead code"
       else
         let num_bytes_sent := conn_response_bytes_sent conn + Z.of_nat r in
         if (num_bytes_sent =? Z.of_nat (String.length (conn_response conn))) then
+          (* The whole message got sent, we start waiting for another
+             message on this connection. *)
           ret {| conn_id := conn_id conn;
                  conn_request := "";
                  conn_response := "";
                  conn_response_bytes_sent := 0;
                  conn_state := RECVING
               |}
-        else 
+        else
+          (* Only part of the message was sent, retry. *)
           ret {| conn_id := conn_id conn;
                  conn_request := conn_request conn;
                  conn_response := conn_response conn;
@@ -167,8 +190,11 @@ Definition conn_write (conn: connection) : M socketE connection :=
                  conn_state := conn_state conn
               |}
      )
+     (* Internal errors can happen, then we discard the connection. *)
      (ret (upd_conn_state conn DELETED)).
 
+(* Call [conn_read] or [conn_write] depending on the state
+   of the connection. *)
 Definition process_conn 
              (buffer_size : Z) (conn: connection) (last_full_msg : string)
           : M socketE (connection * string) :=
@@ -180,6 +206,9 @@ Definition process_conn
   | _ => ret (conn, last_full_msg)
   end.
 
+(* Choose one connection to run [process_conn] with. *)
+(* The returned [bool] is always true and is just waiting to
+   be removed in the next refactoring. *)
 Definition select_loop_body
            (server_addr : endpoint_id)
            (buffer_size : Z)
@@ -196,27 +225,25 @@ Definition select_loop_body
     (let waiting_to_recv := filter (has_conn_state RECVING) connections in
      let waiting_to_send := filter (has_conn_state SENDING) connections in
      conn <- choose (waiting_to_recv ++ waiting_to_send) ;;
-          new_st <- process_conn buffer_size conn last_full_msg ;;
-          let '(conn', last_full_msg') := new_st in
-          let connections' :=
-              replace_when
-                (fun c =>
-                   if (has_conn_state RECVING c
-                       || has_conn_state SENDING c)%bool then 
-                     (conn_id c = conn_id conn' ?)
-                   else
-                     false 
-                )
-                conn'
-                connections in
-          ret (true, (connections', last_full_msg'))
+     new_st <- process_conn buffer_size conn last_full_msg ;;
+     let '(conn', last_full_msg') := new_st in
+     let connections' :=
+         replace_when
+           (fun c =>
+              if (has_conn_state RECVING c
+                  || has_conn_state SENDING c)%bool
+              then (conn_id c = conn_id conn' ?)
+              else false)
+           conn'
+           connections in
+     ret (true, (connections', last_full_msg'))
     ).
 
 Definition select_loop 
                 (server_addr : endpoint_id) (buffer_size : Z)
               : (bool * (list connection * string))
                   -> M socketE (bool * (list connection * string)) :=
-  while fst
+  while fst (* The [while] condition is always true. *)
         (fun '(_, server_st) =>
            select_loop_body server_addr buffer_size server_st).
 
@@ -225,8 +252,9 @@ Definition server_
            (buffer_size : Z)
            (ini_msg : string) :=
   (or (listen endpoint ;;
-       select_loop endpoint buffer_size (true, ([], ini_msg))
-       ;; ret tt)
+       select_loop endpoint buffer_size (true, ([], ini_msg)) ;;
+       ret tt)
+      (* The server can just fail to start during initialization. *)
       (ret tt) ).
 
 Definition server := server_ SERVER_PORT BUFFER_SIZE INIT_MSG.
