dw/DeepWeb/Spec/Trace_Examples.v
@@ -1,0 +1,73 @@
+Generalizable Variable E.
+Typeclasses eauto := 6.
+
+From QuickChick Require Import QuickChick.
+
+Require Import Ascii String List PArith.
+Require Fin.
+Import ListNotations.
+
+From Custom Require Import String.
+
+Require Import DeepWeb.Free.Monad.Free.
+Import MonadNotations.
+Require Import DeepWeb.Free.Monad.Common.
+
+Require Import
+        DeepWeb.Lib.Util
+        DeepWeb.Lib.SimpleSpec
+        DeepWeb.Spec.Swap_SimpleSpec.
+
+(* begin hide *)
+Set Warnings "-extraction-opaque-accessed,-extraction".
+Open Scope string_scope.
+(* end hide *)
+
+Import EventNotations.
+
+(** _Traces_ are lists of "observed events" of the following forms
+    (plus one more that we'll see below):
+<<
+       c !        Connection c is opened
+       c <-- b    Server receives byte b on connection c
+       c --> b    Server sends byte b on connection c
+>>
+*)
+
+(** * Example traces *)
+
+(** The [is_observer_trace_test] property checks that some trace
+    of events belongs to some sequential specification [ObserverM]. *)
+
+(* A simple example illustrated the behavior described by the spec: *)
+Example trace_example :
+  OK tt = is_observer_trace_test swap_observer_def [
+    0 !;
+    1 !;
+    0 <-- "a";
+    0 <-- "b";
+    0 <-- "c";
+    0 --> "0";
+    0 --> "0";
+    0 --> "0";
+    1 <-- "d";
+    1 <-- "e";
+    1 <-- "f";
+    1 --> "a";
+    1 --> "b";
+    1 --> "c"
+  ]%hypo.
+Proof. reflexivity. Qed.
+
+(* An example of a behavior _not_ described by the spec (the first
+   byte sent back should be ["0"], not ["1"]): *)
+Example trace_example2 :
+  FAIL tt = is_observer_trace_test swap_observer_def [
+    0 !;
+    0 <-- "a";
+    0 <-- "b";
+    0 <-- "c";
+    0 --> "1"   (* error: Initial state is 000 *)
+  ]%hypo.
+Proof. reflexivity. Qed.
+
