dw/DeepWeb/Test/TestExternal.v
@@ -208,7 +208,7 @@ Definition execute_prop' (msgs : list byte) : Checker :=
     | [] => collect "No Response" (checker tt) (* If the server never said anything, no point checking. *)
     | _ :: _ => whenFail (show tr)
       (is_scrambled_trace_test
-         5000 Swap_SimpleSpec.swap_observer_def tr)
+         Swap_SimpleSpec.swap_observer_def tr)
     end
   end.
 
